chore: cleanup

src/Std/Data/DList.lean
@@ -12,57 +12,61 @@ This structure supports `O(1)` `append` and `concat` operations on lists, making
 useful for append-heavy uses such as logging and pretty printing.
 -/
 structure DList (α : Type u) :=
-(apply     : List α → List α)
-(invariant : ∀ l, apply l = apply [] ++ l)
+  (apply     : List α → List α)
+  (invariant : ∀ l, apply l = apply [] ++ l)
 
 namespace DList
 variables {α : Type u}
 open List
 
 def ofList (l : List α) : DList α :=
-⟨Append.append l, fun t => by rw appendNil; exact rfl⟩
+  ⟨Append.append l, fun t => by rw appendNil; exact rfl⟩
 
 def empty : DList α :=
-⟨id, fun t => rfl⟩
+  ⟨id, fun t => rfl⟩
 
 instance : EmptyCollection (DList α) :=
-⟨DList.empty⟩
+  ⟨DList.empty⟩
 
 def toList : DList α → List α
-| ⟨f, h⟩ => f []
+  | ⟨f, h⟩ => f []
 
-def singleton (a : α) : DList α :=
-⟨fun t => a :: t,
- fun t => rfl⟩
+def singleton (a : α) : DList α := {
+  apply     := fun t => a :: t,
+  invariant := fun t => rfl
+}
 
 def cons : α → DList α → DList α
-| a, ⟨f, h⟩ =>
-  ⟨fun t => a :: f t,
-   fun t =>
-    show a :: f t = a :: f [] ++ t from
-    have h₁ : a :: f t = a :: (f nil ++ t) by rw h t; exact rfl
-    have h₂ : a :: (f nil ++ t) = a :: f nil ++ t := (consAppend _ _ _).symm
-    Eq.trans h₁ h₂⟩
+  | a, ⟨f, h⟩ => {
+    apply     := fun t => a :: f t,
+    invariant := by
+      intro t
+      show a :: f t = a :: f [] ++ t
+      rw [consAppend, h]
+      exact rfl
+  }
 
 def append : DList α → DList α → DList α
-| ⟨f, h₁⟩, ⟨g, h₂⟩ =>
-  ⟨f ∘ g, by
-    intro t
-    show f (g t) = (f (g [])) ++ t
-    rw [h₁ (g t), h₂ t, ← appendAssoc (f []) (g []) t, ← h₁ (g [])]
-    exact rfl⟩
+  | ⟨f, h₁⟩, ⟨g, h₂⟩ => {
+    apply     := f ∘ g,
+    invariant := by
+      intro t
+      show f (g t) = (f (g [])) ++ t
+      rw [h₁ (g t), h₂ t, ← appendAssoc (f []) (g []) t, ← h₁ (g [])]
+      exact rfl
+    }
 
 def push : DList α → α → DList α
-| ⟨f, h⟩, a =>
-  ⟨fun t => f (a :: t),
-   by
-    intro t
-    show f (a :: t) = f (a :: nil) ++ t
-    rw [h [a], h (a::t), appendAssoc (f []) [a] t]
-    exact rfl⟩
+  | ⟨f, h⟩, a => {
+    apply     := fun t => f (a :: t),
+    invariant := by
+      intro t
+      show f (a :: t) = f (a :: nil) ++ t
+      rw [h [a], h (a::t), appendAssoc (f []) [a] t]
+      exact rfl
+  }
 
-instance : Append (DList α) :=
-⟨DList.append⟩
+instance : Append (DList α) := ⟨DList.append⟩
 
 end DList
 end Std
