src/Std/Data/AssocList.lean
@@ -8,87 +8,87 @@ namespace Std
 
 /- List-like type to avoid extra level of indirection -/
 inductive AssocList (α : Type u) (β : Type v)
-| nil : AssocList α β
-| cons (key : α) (value : β) (tail : AssocList α β) : AssocList α β
+  | nil : AssocList α β
+  | cons (key : α) (value : β) (tail : AssocList α β) : AssocList α β
 
 namespace AssocList
 variables {α : Type u} {β : Type v} {δ : Type w} {m : Type w → Type w} [Monad m]
 
 abbrev empty : AssocList α β :=
-nil
+  nil
 
 instance : EmptyCollection (AssocList α β) := ⟨empty⟩
 
 abbrev insert (m : AssocList α β) (k : α) (v : β) : AssocList α β :=
-m.cons k v
+  m.cons k v
 
 def isEmpty : AssocList α β → Bool
-| nil => true
-| _   => false
+  | nil => true
+  | _   => false
 
 @[specialize] def foldlM (f : δ → α → β → m δ) : (init : δ) → AssocList α β → m δ
-| d, nil         => pure d
-| d, cons a b es => do d ← f d a b; foldlM f d es
+  | d, nil         => pure d
+  | d, cons a b es => do d ← f d a b; foldlM f d es
 
 @[inline] def foldl (f : δ → α → β → δ) (init : δ) (as : AssocList α β) : δ :=
-Id.run (foldlM f init as)
+  Id.run (foldlM f init as)
 
 def mapKey (f : α → δ) : AssocList α β → AssocList δ β
-| nil        => nil
-| cons k v t => cons (f k) v (mapKey f t)
+  | nil        => nil
+  | cons k v t => cons (f k) v (mapKey f t)
 
 def mapVal (f : β → δ) : AssocList α β → AssocList α δ
-| nil        => nil
-| cons k v t => cons k (f v) (mapVal f t)
+  | nil        => nil
+  | cons k v t => cons k (f v) (mapVal f t)
 
 def findEntry? [BEq α] (a : α) : AssocList α β → Option (α × β)
-| nil         => none
-| cons k v es => match k == a with
-  | true  => some (k, v)
-  | false => findEntry? a es
+  | nil         => none
+  | cons k v es => match k == a with
+    | true  => some (k, v)
+    | false => findEntry? a es
 
 def find? [BEq α] (a : α) : AssocList α β → Option β
-| nil         => none
-| cons k v es => match k == a with
-  | true  => some v
-  | false => find? a es
+  | nil         => none
+  | cons k v es => match k == a with
+    | true  => some v
+    | false => find? a es
 
 def contains [BEq α] (a : α) : AssocList α β → Bool
-| nil         => false
-| cons k v es => k == a || contains a es
+  | nil         => false
+  | cons k v es => k == a || contains a es
 
 def replace [BEq α] (a : α) (b : β) : AssocList α β → AssocList α β
-| nil         => nil
-| cons k v es => match k == a with
-  | true  => cons a b es
-  | false => cons k v (replace a b es)
+  | nil         => nil
+  | cons k v es => match k == a with
+    | true  => cons a b es
+    | false => cons k v (replace a b es)
 
 def erase [BEq α] (a : α) : AssocList α β → AssocList α β
-| nil         => nil
-| cons k v es => match k == a with
-  | true  => es
-  | false => cons k v (erase a es)
+  | nil         => nil
+  | cons k v es => match k == a with
+    | true  => es
+    | false => cons k v (erase a es)
 
 def any (p : α → β → Bool) : AssocList α β → Bool
-| nil         => false
-| cons k v es => p k v || any p es
+  | nil         => false
+  | cons k v es => p k v || any p es
 
 def all (p : α → β → Bool) : AssocList α β → Bool
-| nil         => true
-| cons k v es => p k v && all p es
+  | nil         => true
+  | cons k v es => p k v && all p es
 
 @[inline] def forIn {α : Type u} {β : Type v} {δ : Type w} {m : Type w → Type w'} [Monad m]
     (as : AssocList α β) (init : δ) (f : (α × β) → δ → m (ForInStep δ)) : m δ :=
-let rec @[specialize] loop
-  | d, nil => pure d
-  | d, cons k v es => do
-    match (← f (k, v) d) with
-    | ForInStep.done d  => pure d
-    | ForInStep.yield d => loop d es
-loop init as
+  let rec @[specialize] loop
+    | d, nil => pure d
+    | d, cons k v es => do
+      match (← f (k, v) d) with
+      | ForInStep.done d  => pure d
+      | ForInStep.yield d => loop d es
+  loop init as
 
 end Std.AssocList
 
 def List.toAssocList {α : Type u} {β : Type v} : List (α × β) → Std.AssocList α β
-| []          => Std.AssocList.nil
-| (a,b) :: es => Std.AssocList.cons a b (toAssocList es)
+  | []          => Std.AssocList.nil
+  | (a,b) :: es => Std.AssocList.cons a b (toAssocList es)
