src/Std/Data/PersistentHashMap.lean
@@ -9,17 +9,17 @@ universes u v w w'
 namespace PersistentHashMap
 
 inductive Entry (α : Type u) (β : Type v) (σ : Type w)
-| entry (key : α) (val : β) : Entry α β σ
-| ref   (node : σ) : Entry α β σ
-| null  : Entry α β σ
+  | entry (key : α) (val : β) : Entry α β σ
+  | ref   (node : σ) : Entry α β σ
+  | null  : Entry α β σ
 
-instance Entry.inhabited {α β σ} : Inhabited (Entry α β σ) := ⟨Entry.null⟩
+instance {α β σ} : Inhabited (Entry α β σ) := ⟨Entry.null⟩
 
 inductive Node (α : Type u) (β : Type v) : Type (max u v)
-| entries   (es : Array (Entry α β (Node α β))) : Node α β
-| collision (ks : Array α) (vs : Array β) (h : ks.size = vs.size) : Node α β
+  | entries   (es : Array (Entry α β (Node α β))) : Node α β
+  | collision (ks : Array α) (vs : Array β) (h : ks.size = vs.size) : Node α β
 
-instance Node.inhabited {α β} : Inhabited (Node α β) := ⟨Node.entries #[]⟩
+instance {α β} : Inhabited (Node α β) := ⟨Node.entries #[]⟩
 
 abbrev shift         : USize  := 5
 abbrev branching     : USize  := USize.ofNat (2 ^ shift.toNat)
@@ -27,13 +27,13 @@ abbrev maxDepth      : USize  := 7
 abbrev maxCollisions : Nat    := 4
 
 def mkEmptyEntriesArray {α β} : Array (Entry α β (Node α β)) :=
-(Array.mkArray PersistentHashMap.branching.toNat PersistentHashMap.Entry.null)
+  (Array.mkArray PersistentHashMap.branching.toNat PersistentHashMap.Entry.null)
 
 end PersistentHashMap
 
 structure PersistentHashMap (α : Type u) (β : Type v) [BEq α] [Hashable α] :=
-(root    : PersistentHashMap.Node α β := PersistentHashMap.Node.entries PersistentHashMap.mkEmptyEntriesArray)
-(size    : Nat                        := 0)
+  (root    : PersistentHashMap.Node α β := PersistentHashMap.Node.entries PersistentHashMap.mkEmptyEntriesArray)
+  (size    : Nat                        := 0)
 
 abbrev PHashMap (α : Type u) (β : Type v) [BEq α] [Hashable α] := PersistentHashMap α β
 
@@ -43,98 +43,94 @@ variables {α : Type u} {β : Type v}
 def empty [BEq α] [Hashable α] : PersistentHashMap α β := {}
 
 def isEmpty [BEq α] [Hashable α] (m : PersistentHashMap α β) : Bool :=
-m.size == 0
+  m.size == 0
 
 instance [BEq α] [Hashable α] : Inhabited (PersistentHashMap α β) := ⟨{}⟩
 
 def mkEmptyEntries {α β} : Node α β :=
-Node.entries mkEmptyEntriesArray
+  Node.entries mkEmptyEntriesArray
 
 abbrev mul2Shift (i : USize) (shift : USize) : USize := i.shiftLeft shift
 abbrev div2Shift (i : USize) (shift : USize) : USize := i.shiftRight shift
 abbrev mod2Shift (i : USize) (shift : USize) : USize := USize.land i ((USize.shiftLeft 1 shift) - 1)
 
 inductive IsCollisionNode : Node α β → Prop
-| mk (keys : Array α) (vals : Array β) (h : keys.size = vals.size) : IsCollisionNode (Node.collision keys vals h)
+  | mk (keys : Array α) (vals : Array β) (h : keys.size = vals.size) : IsCollisionNode (Node.collision keys vals h)
 
 abbrev CollisionNode (α β) := { n : Node α β // IsCollisionNode n }
 
 inductive IsEntriesNode : Node α β → Prop
-| mk (entries : Array (Entry α β (Node α β))) : IsEntriesNode (Node.entries entries)
+  | mk (entries : Array (Entry α β (Node α β))) : IsEntriesNode (Node.entries entries)
 
 abbrev EntriesNode (α β) := { n : Node α β // IsEntriesNode n }
 
 private theorem setSizeEq {ks : Array α} {vs : Array β} (h : ks.size = vs.size) (i : Fin ks.size) (j : Fin vs.size) (k : α) (v : β)
-                           : (ks.set i k).size = (vs.set j v).size :=
-have h₁ : (ks.set i k).size = ks.size by apply Array.szFSetEq
-have h₂ : (vs.set j v).size = vs.size by apply Array.szFSetEq
-(h₁.trans h).trans h₂.symm
+                           : (ks.set i k).size = (vs.set j v).size := by
+  rw [Array.szFSetEq, Array.szFSetEq vs, h]
+  exact rfl
 
-private theorem pushSizeEq {ks : Array α} {vs : Array β} (h : ks.size = vs.size) (k : α) (v : β) : (ks.push k).size = (vs.push v).size :=
-have h₁ : (ks.push k).size = ks.size + 1 by apply Array.szPushEq
-have h₂ : (vs.push v).size = vs.size + 1 by apply Array.szPushEq
-have h₃ : ks.size + 1 = vs.size + 1      by rw h; exact rfl
-(h₁.trans h₃).trans h₂.symm
+private theorem pushSizeEq {ks : Array α} {vs : Array β} (h : ks.size = vs.size) (k : α) (v : β) : (ks.push k).size = (vs.push v).size := by
+  rw [Array.szPushEq, Array.szPushEq, h]
+  exact rfl
 
 partial def insertAtCollisionNodeAux [BEq α] : CollisionNode α β → Nat → α → β → CollisionNode α β
-| n@⟨Node.collision keys vals heq, _⟩, i, k, v =>
-  if h : i < keys.size then
-    let idx : Fin keys.size := ⟨i, h⟩;
-    let k' := keys.get idx;
-    if k == k' then
-       let j : Fin vals.size := ⟨i, by rw [←heq]; assumption⟩
-       ⟨Node.collision (keys.set idx k) (vals.set j v) (setSizeEq heq idx j k v), IsCollisionNode.mk _ _ _⟩
-    else insertAtCollisionNodeAux n (i+1) k v
-  else
-    ⟨Node.collision (keys.push k) (vals.push v) (pushSizeEq heq k v), IsCollisionNode.mk _ _ _⟩
-| ⟨Node.entries _, h⟩, _, _, _ => False.elim (nomatch h)
+  | n@⟨Node.collision keys vals heq, _⟩, i, k, v =>
+    if h : i < keys.size then
+      let idx : Fin keys.size := ⟨i, h⟩;
+      let k' := keys.get idx;
+      if k == k' then
+         let j : Fin vals.size := ⟨i, by rw [←heq]; assumption⟩
+         ⟨Node.collision (keys.set idx k) (vals.set j v) (setSizeEq heq idx j k v), IsCollisionNode.mk _ _ _⟩
+      else insertAtCollisionNodeAux n (i+1) k v
+    else
+      ⟨Node.collision (keys.push k) (vals.push v) (pushSizeEq heq k v), IsCollisionNode.mk _ _ _⟩
+  | ⟨Node.entries _, h⟩, _, _, _ => False.elim (nomatch h)
 
 def insertAtCollisionNode [BEq α] : CollisionNode α β → α → β → CollisionNode α β :=
-fun n k v => insertAtCollisionNodeAux n 0 k v
+  fun n k v => insertAtCollisionNodeAux n 0 k v
 
 def getCollisionNodeSize : CollisionNode α β → Nat
-| ⟨Node.collision keys _ _, _⟩ => keys.size
-| ⟨Node.entries _, h⟩          => False.elim (nomatch h)
+  | ⟨Node.collision keys _ _, _⟩ => keys.size
+  | ⟨Node.entries _, h⟩          => False.elim (nomatch h)
 
 def mkCollisionNode (k₁ : α) (v₁ : β) (k₂ : α) (v₂ : β) : Node α β :=
-let ks : Array α := Array.mkEmpty maxCollisions
-let ks := (ks.push k₁).push k₂
-let vs : Array β := Array.mkEmpty maxCollisions
-let vs := (vs.push v₁).push v₂
-Node.collision ks vs rfl
+  let ks : Array α := Array.mkEmpty maxCollisions
+  let ks := (ks.push k₁).push k₂
+  let vs : Array β := Array.mkEmpty maxCollisions
+  let vs := (vs.push v₁).push v₂
+  Node.collision ks vs rfl
 
 partial def insertAux [BEq α] [Hashable α] : Node α β → USize → USize → α → β → Node α β
-| Node.collision keys vals heq, _, depth, k, v =>
-  let newNode := insertAtCollisionNode ⟨Node.collision keys vals heq, IsCollisionNode.mk _ _ _⟩ k v
-  if depth >= maxDepth || getCollisionNodeSize newNode < maxCollisions then newNode.val
-  else match newNode with
-    | ⟨Node.entries _, h⟩ => False.elim (nomatch h)
-    | ⟨Node.collision keys vals heq, _⟩ =>
-      let rec traverse (i : Nat) (entries : Node α β) : Node α β :=
-        if h : i < keys.size then
-          let k := keys.get ⟨i, h⟩
-          let v := vals.get ⟨i, heq ▸ h⟩
-          let h := hash k
-          let h := div2Shift h (shift * (depth - 1))
-          traverse (i+1) (insertAux entries h depth k v)
-        else
-          entries
-      traverse 0 mkEmptyEntries
-| Node.entries entries, h, depth, k, v =>
-  let j     := (mod2Shift h shift).toNat
-  Node.entries $ entries.modify j fun entry =>
-    match entry with
-    | Entry.null        => Entry.entry k v
-    | Entry.ref node    => Entry.ref $ insertAux node (div2Shift h shift) (depth+1) k v
-    | Entry.entry k' v' =>
-      if k == k' then Entry.entry k v
-      else Entry.ref $ mkCollisionNode k' v' k v
+  | Node.collision keys vals heq, _, depth, k, v =>
+    let newNode := insertAtCollisionNode ⟨Node.collision keys vals heq, IsCollisionNode.mk _ _ _⟩ k v
+    if depth >= maxDepth || getCollisionNodeSize newNode < maxCollisions then newNode.val
+    else match newNode with
+      | ⟨Node.entries _, h⟩ => False.elim (nomatch h)
+      | ⟨Node.collision keys vals heq, _⟩ =>
+        let rec traverse (i : Nat) (entries : Node α β) : Node α β :=
+          if h : i < keys.size then
+            let k := keys.get ⟨i, h⟩
+            let v := vals.get ⟨i, heq ▸ h⟩
+            let h := hash k
+            let h := div2Shift h (shift * (depth - 1))
+            traverse (i+1) (insertAux entries h depth k v)
+          else
+            entries
+        traverse 0 mkEmptyEntries
+  | Node.entries entries, h, depth, k, v =>
+    let j     := (mod2Shift h shift).toNat
+    Node.entries $ entries.modify j fun entry =>
+      match entry with
+      | Entry.null        => Entry.entry k v
+      | Entry.ref node    => Entry.ref $ insertAux node (div2Shift h shift) (depth+1) k v
+      | Entry.entry k' v' =>
+        if k == k' then Entry.entry k v
+        else Entry.ref $ mkCollisionNode k' v' k v
 
 def insert [BEq α] [Hashable α] : PersistentHashMap α β → α → β → PersistentHashMap α β
-| { root := n, size := sz }, k, v => { root := insertAux n (hash k) 1 k v, size := sz + 1 }
+  | { root := n, size := sz }, k, v => { root := insertAux n (hash k) 1 k v, size := sz + 1 }
 
-partial def findAtAux [BEq α] (keys : Array α) (vals : Array β) (heq : keys.size = vals.size) : Nat → α → Option β
-| i, k =>
+partial def findAtAux [BEq α] (keys : Array α) (vals : Array β) (heq : keys.size = vals.size) (i : Nat) (k : α) : Option β :=
   if h : i < keys.size then
     let k' := keys.get ⟨i, h⟩
     if k == k' then some (vals.get ⟨i, by rw [←heq]; assumption⟩)
@@ -142,30 +138,29 @@ partial def findAtAux [BEq α] (keys : Array α) (vals : Array β) (heq : keys.s
   else none
 
 partial def findAux [BEq α] : Node α β → USize → α → Option β
-| Node.entries entries, h, k =>
-  let j     := (mod2Shift h shift).toNat
-  match entries.get! j with
-  | Entry.null       => none
-  | Entry.ref node   => findAux node (div2Shift h shift) k
-  | Entry.entry k' v => if k == k' then some v else none
-| Node.collision keys vals heq, _, k => findAtAux keys vals heq 0 k
+  | Node.entries entries, h, k =>
+    let j     := (mod2Shift h shift).toNat
+    match entries.get! j with
+    | Entry.null       => none
+    | Entry.ref node   => findAux node (div2Shift h shift) k
+    | Entry.entry k' v => if k == k' then some v else none
+  | Node.collision keys vals heq, _, k => findAtAux keys vals heq 0 k
 
 def find? [BEq α] [Hashable α] : PersistentHashMap α β → α → Option β
-| { root := n, .. }, k => findAux n (hash k) k
+  | { root := n, .. }, k => findAux n (hash k) k
 
 @[inline] def getOp [BEq α] [Hashable α] (self : PersistentHashMap α β) (idx : α) : Option β :=
-self.find? idx
+  self.find? idx
 
 @[inline] def findD [BEq α] [Hashable α] (m : PersistentHashMap α β) (a : α) (b₀ : β) : β :=
-(m.find? a).getD b₀
+  (m.find? a).getD b₀
 
 @[inline] def find! [BEq α] [Hashable α] [Inhabited β] (m : PersistentHashMap α β) (a : α) : β :=
-match m.find? a with
-| some b => b
-| none   => panic! "key is not in the map"
+  match m.find? a with
+  | some b => b
+  | none   => panic! "key is not in the map"
 
-partial def findEntryAtAux [BEq α] (keys : Array α) (vals : Array β) (heq : keys.size = vals.size) : Nat → α → Option (α × β)
-| i, k =>
+partial def findEntryAtAux [BEq α] (keys : Array α) (vals : Array β) (heq : keys.size = vals.size) (i : Nat) (k : α) : Option (α × β) :=
   if h : i < keys.size then
     let k' := keys.get ⟨i, h⟩
     if k == k' then some (k', vals.get ⟨i, by rw [←heq]; assumption⟩)
@@ -173,19 +168,18 @@ partial def findEntryAtAux [BEq α] (keys : Array α) (vals : Array β) (heq : k
   else none
 
 partial def findEntryAux [BEq α] : Node α β → USize → α → Option (α × β)
-| Node.entries entries, h, k =>
-  let j     := (mod2Shift h shift).toNat
-  match entries.get! j with
-  | Entry.null       => none
-  | Entry.ref node   => findEntryAux node (div2Shift h shift) k
-  | Entry.entry k' v => if k == k' then some (k', v) else none
-| Node.collision keys vals heq, _, k => findEntryAtAux keys vals heq 0 k
+  | Node.entries entries, h, k =>
+    let j     := (mod2Shift h shift).toNat
+    match entries.get! j with
+    | Entry.null       => none
+    | Entry.ref node   => findEntryAux node (div2Shift h shift) k
+    | Entry.entry k' v => if k == k' then some (k', v) else none
+  | Node.collision keys vals heq, _, k => findEntryAtAux keys vals heq 0 k
 
 def findEntry? [BEq α] [Hashable α] : PersistentHashMap α β → α → Option (α × β)
-| { root := n, .. }, k => findEntryAux n (hash k) k
+  | { root := n, .. }, k => findEntryAux n (hash k) k
 
-partial def containsAtAux [BEq α] (keys : Array α) (vals : Array β) (heq : keys.size = vals.size) : Nat → α → Bool
-| i, k =>
+partial def containsAtAux [BEq α] (keys : Array α) (vals : Array β) (heq : keys.size = vals.size) (i : Nat) (k : α) : Bool :=
   if h : i < keys.size then
     let k' := keys.get ⟨i, h⟩
     if k == k' then true
@@ -193,19 +187,18 @@ partial def containsAtAux [BEq α] (keys : Array α) (vals : Array β) (heq : ke
   else false
 
 partial def containsAux [BEq α] : Node α β → USize → α → Bool
-| Node.entries entries, h, k =>
-  let j     := (mod2Shift h shift).toNat
-  match entries.get! j with
-  | Entry.null       => false
-  | Entry.ref node   => containsAux node (div2Shift h shift) k
-  | Entry.entry k' v => k == k'
-| Node.collision keys vals heq, _, k => containsAtAux keys vals heq 0 k
+  | Node.entries entries, h, k =>
+    let j     := (mod2Shift h shift).toNat
+    match entries.get! j with
+    | Entry.null       => false
+    | Entry.ref node   => containsAux node (div2Shift h shift) k
+    | Entry.entry k' v => k == k'
+  | Node.collision keys vals heq, _, k => containsAtAux keys vals heq 0 k
 
 def contains [BEq α] [Hashable α] : PersistentHashMap α β → α → Bool
-| { root := n, .. }, k => containsAux n (hash k) k
+  | { root := n, .. }, k => containsAux n (hash k) k
 
-partial def isUnaryEntries (a : Array (Entry α β (Node α β))) : Nat → Option (α × β) → Option (α × β)
-| i, acc =>
+partial def isUnaryEntries (a : Array (Entry α β (Node α β))) (i : Nat) (acc : Option (α × β)) : Option (α × β) :=
   if h : i < a.size then
     match a.get ⟨i, h⟩ with
     | Entry.null      => isUnaryEntries a (i+1) acc
@@ -217,107 +210,107 @@ partial def isUnaryEntries (a : Array (Entry α β (Node α β))) : Nat → Opti
   else acc
 
 def isUnaryNode : Node α β → Option (α × β)
-| Node.entries entries         => isUnaryEntries entries 0 none
-| Node.collision keys vals heq =>
-  if h : 1 = keys.size then
-    have 0 < keys.size by rw [←h]; exact decide!
-    some (keys.get ⟨0, this⟩, vals.get ⟨0, by rw [←heq]; assumption⟩)
-  else
-    none
+  | Node.entries entries         => isUnaryEntries entries 0 none
+  | Node.collision keys vals heq =>
+    if h : 1 = keys.size then
+      have 0 < keys.size by rw [←h]; exact decide!
+      some (keys.get ⟨0, this⟩, vals.get ⟨0, by rw [←heq]; assumption⟩)
+    else
+      none
 
 partial def eraseAux [BEq α] : Node α β → USize → α → Node α β × Bool
-| n@(Node.collision keys vals heq), _, k =>
-  match keys.indexOf? k with
-  | some idx =>
-    let ⟨keys', keq⟩ := keys.eraseIdx' idx
-    let ⟨vals', veq⟩ := vals.eraseIdx' (Eq.ndrec idx heq)
-    have keys.size - 1 = vals.size - 1 by rw [heq]; exact rfl
-    (Node.collision keys' vals' (keq.trans (this.trans veq.symm)), true)
-  | none     => (n, false)
-| n@(Node.entries entries), h, k =>
-  let j       := (mod2Shift h shift).toNat
-  let entry   := entries.get! j
-  match entry with
-  | Entry.null       => (n, false)
-  | Entry.entry k' v =>
-    if k == k' then (Node.entries (entries.set! j Entry.null), true) else (n, false)
-  | Entry.ref node   =>
-    let entries := entries.set! j Entry.null
-    let (newNode, deleted) := eraseAux node (div2Shift h shift) k
-    if !deleted then (n, false)
-    else match isUnaryNode newNode with
-      | none        => (Node.entries (entries.set! j (Entry.ref newNode)), true)
-      | some (k, v) => (Node.entries (entries.set! j (Entry.entry k v)), true)
+  | n@(Node.collision keys vals heq), _, k =>
+    match keys.indexOf? k with
+    | some idx =>
+      let ⟨keys', keq⟩ := keys.eraseIdx' idx
+      let ⟨vals', veq⟩ := vals.eraseIdx' (Eq.ndrec idx heq)
+      have keys.size - 1 = vals.size - 1 by rw [heq]; exact rfl
+      (Node.collision keys' vals' (keq.trans (this.trans veq.symm)), true)
+    | none     => (n, false)
+  | n@(Node.entries entries), h, k =>
+    let j       := (mod2Shift h shift).toNat
+    let entry   := entries.get! j
+    match entry with
+    | Entry.null       => (n, false)
+    | Entry.entry k' v =>
+      if k == k' then (Node.entries (entries.set! j Entry.null), true) else (n, false)
+    | Entry.ref node   =>
+      let entries := entries.set! j Entry.null
+      let (newNode, deleted) := eraseAux node (div2Shift h shift) k
+      if !deleted then (n, false)
+      else match isUnaryNode newNode with
+        | none        => (Node.entries (entries.set! j (Entry.ref newNode)), true)
+        | some (k, v) => (Node.entries (entries.set! j (Entry.entry k v)), true)
 
 def erase [BEq α] [Hashable α] : PersistentHashMap α β → α → PersistentHashMap α β
-| { root := n, size := sz }, k =>
-  let h := hash k
-  let (n, del) := eraseAux n h k
-  { root := n, size := if del then sz - 1 else sz }
+  | { root := n, size := sz }, k =>
+    let h := hash k
+    let (n, del) := eraseAux n h k
+    { root := n, size := if del then sz - 1 else sz }
 
 section
 variables {m : Type w → Type w'} [Monad m]
 variables {σ : Type w}
 
 @[specialize] partial def foldlMAux (f : σ → α → β → m σ) : Node α β → σ → m σ
-| Node.collision keys vals heq, acc =>
-  let rec traverse (i : Nat) (acc : σ) : m σ := do
-    if h : i < keys.size then
-      let k := keys.get ⟨i, h⟩
-      let v := vals.get ⟨i, heq ▸ h⟩
-      traverse (i+1) (← f acc k v)
-    else
-      pure acc
-  traverse 0 acc
-| Node.entries entries, acc => entries.foldlM (fun acc entry =>
-  match entry with
-  | Entry.null      => pure acc
-  | Entry.entry k v => f acc k v
-  | Entry.ref node  => foldlMAux f node acc)
-  acc
+  | Node.collision keys vals heq, acc =>
+    let rec traverse (i : Nat) (acc : σ) : m σ := do
+      if h : i < keys.size then
+        let k := keys.get ⟨i, h⟩
+        let v := vals.get ⟨i, heq ▸ h⟩
+        traverse (i+1) (← f acc k v)
+      else
+        pure acc
+    traverse 0 acc
+  | Node.entries entries, acc => entries.foldlM (fun acc entry =>
+    match entry with
+    | Entry.null      => pure acc
+    | Entry.entry k v => f acc k v
+    | Entry.ref node  => foldlMAux f node acc)
+    acc
 
-@[specialize] def foldlM [BEq α] [Hashable α] (map : PersistentHashMap α β) (f : σ → α → β → m σ) (acc : σ) : m σ :=
-foldlMAux f map.root acc
+@[specialize] def foldlM [BEq α] [Hashable α] (map : PersistentHashMap α β) (f : σ → α → β → m σ) (init : σ) : m σ :=
+  foldlMAux f map.root init
 
 @[specialize] def forM [BEq α] [Hashable α] (map : PersistentHashMap α β) (f : α → β → m PUnit) : m PUnit :=
-map.foldlM (fun _ => f) ⟨⟩
+  map.foldlM (fun _ => f) ⟨⟩
 
-@[specialize] def foldl [BEq α] [Hashable α] (map : PersistentHashMap α β) (f : σ → α → β → σ) (acc : σ) : σ :=
-Id.run $ map.foldlM f acc
+@[specialize] def foldl [BEq α] [Hashable α] (map : PersistentHashMap α β) (f : σ → α → β → σ) (init : σ) : σ :=
+  Id.run $ map.foldlM f init
 end
 
 def toList [BEq α] [Hashable α] (m : PersistentHashMap α β) : List (α × β) :=
-m.foldl (fun ps k v => (k, v) :: ps) []
+  m.foldl (init := []) fun ps k v => (k, v) :: ps
 
 structure Stats :=
-(numNodes      : Nat := 0)
-(numNull       : Nat := 0)
-(numCollisions : Nat := 0)
-(maxDepth      : Nat := 0)
+  (numNodes      : Nat := 0)
+  (numNull       : Nat := 0)
+  (numCollisions : Nat := 0)
+  (maxDepth      : Nat := 0)
 
 partial def collectStats : Node α β → Stats → Nat → Stats
-| Node.collision keys _ _, stats, depth =>
-  { stats with
-    numNodes      := stats.numNodes + 1,
-    numCollisions := stats.numCollisions + keys.size - 1,
-    maxDepth      := Nat.max stats.maxDepth depth }
-| Node.entries entries, stats, depth =>
-  let stats :=
+  | Node.collision keys _ _, stats, depth =>
     { stats with
       numNodes      := stats.numNodes + 1,
+      numCollisions := stats.numCollisions + keys.size - 1,
       maxDepth      := Nat.max stats.maxDepth depth }
-  entries.foldl (fun stats entry =>
-    match entry with
-    | Entry.null      => { stats with numNull := stats.numNull + 1 }
-    | Entry.ref node  => collectStats node stats (depth + 1)
-    | Entry.entry _ _ => stats)
-    stats
+  | Node.entries entries, stats, depth =>
+    let stats :=
+      { stats with
+        numNodes      := stats.numNodes + 1,
+        maxDepth      := Nat.max stats.maxDepth depth }
+    entries.foldl (fun stats entry =>
+      match entry with
+      | Entry.null      => { stats with numNull := stats.numNull + 1 }
+      | Entry.ref node  => collectStats node stats (depth + 1)
+      | Entry.entry _ _ => stats)
+      stats
 
 def stats [BEq α] [Hashable α] (m : PersistentHashMap α β) : Stats :=
-collectStats m.root {} 1
+  collectStats m.root {} 1
 
 def Stats.toString (s : Stats) : String :=
-s!"\{ nodes := {s.numNodes}, null := {s.numNull}, collisions := {s.numCollisions}, depth := {s.maxDepth}}"
+  s!"\{ nodes := {s.numNodes}, null := {s.numNull}, collisions := {s.numCollisions}, depth := {s.maxDepth}}"
 
 instance : ToString Stats := ⟨Stats.toString⟩
 
