src/Std/Data/PersistentHashSet.lean
@@ -9,7 +9,7 @@ namespace Std
 universes u v
 
 structure PersistentHashSet (α : Type u) [BEq α] [Hashable α] :=
-(set : PersistentHashMap α Unit)
+  (set : PersistentHashMap α Unit)
 
 abbrev PHashSet (α : Type u) [BEq α] [Hashable α] := PersistentHashSet α
 
@@ -18,39 +18,39 @@ namespace PersistentHashSet
 variables {α : Type u} [BEq α] [Hashable α]
 
 @[inline] def isEmpty (s : PersistentHashSet α) : Bool :=
-s.set.isEmpty
+  s.set.isEmpty
 
 @[inline] def empty : PersistentHashSet α :=
-{ set := PersistentHashMap.empty }
+  { set := PersistentHashMap.empty }
 
 instance : Inhabited (PersistentHashSet α) :=
-⟨empty⟩
+  ⟨empty⟩
 
 instance : EmptyCollection (PersistentHashSet α) :=
-⟨empty⟩
+  ⟨empty⟩
 
 @[inline] def insert (s : PersistentHashSet α) (a : α) : PersistentHashSet α :=
-{ set := s.set.insert a () }
+  { set := s.set.insert a () }
 
 @[inline] def erase (s : PersistentHashSet α) (a : α) : PersistentHashSet α :=
-{ set := s.set.erase a }
+  { set := s.set.erase a }
 
 @[inline] def find? (s : PersistentHashSet α) (a : α) : Option α :=
-match s.set.findEntry? a with
-| some (a, _) => some a
-| none        => none
+  match s.set.findEntry? a with
+  | some (a, _) => some a
+  | none        => none
 
 @[inline] def contains (s : PersistentHashSet α) (a : α) : Bool :=
-s.set.contains a
+  s.set.contains a
 
 @[inline] def size (s : PersistentHashSet α) : Nat :=
-s.set.size
+  s.set.size
 
-@[inline] def foldM {β : Type v} {m : Type v → Type v} [Monad m] (f : β → α → m β) (d : β) (s : PersistentHashSet α) : m β :=
-s.set.foldlM (fun d a _ => f d a) d
+@[inline] def foldM {β : Type v} {m : Type v → Type v} [Monad m] (f : β → α → m β) (init : β) (s : PersistentHashSet α) : m β :=
+  s.set.foldlM (init := init) fun d a _ => f d a
 
-@[inline] def fold {β : Type v} (f : β → α → β) (d : β) (s : PersistentHashSet α) : β :=
-Id.run $ s.foldM f d
+@[inline] def fold {β : Type v} (f : β → α → β) (init : β) (s : PersistentHashSet α) : β :=
+  Id.run $ s.foldM f init
 
 end PersistentHashSet
 end Std
